Bignum: Add more tests; syntax cleanup

Bignum/Component/Extra.lean
@@ -45,16 +45,17 @@ def tophalf {w : Nat} : Component (BitVec w) (BitVec (w.succ / 2)) :=
 Components for subwords of bitvectors with a specific length.
 -/
 def bottom_256 : Component (BitVec 512) (BitVec 256) := @bottomhalf 512
-def top_256    : Component (BitVec 512) (BitVec 256) := @tophalf 512
 def bottom_128 : Component (BitVec 256) (BitVec 128) := @bottomhalf 256
-def top_128    : Component (BitVec 256) (BitVec 128) := @tophalf 256
 def bottom_64  : Component (BitVec 128) (BitVec 64)  := @bottomhalf 128
-def top_64     : Component (BitVec 128) (BitVec 64)  := @tophalf 128
 def bottom_32  : Component (BitVec 64) (BitVec 32)   := @bottomhalf 64
-def top_32     : Component (BitVec 64) (BitVec 32)   := @tophalf 64
 def bottom_16  : Component (BitVec 32) (BitVec 16)   := @bottomhalf 32
-def top_16     : Component (BitVec 32) (BitVec 16)   := @tophalf 32
 def bottom_8   : Component (BitVec 16) (BitVec 8)    := @bottomhalf 16
+
+def top_256    : Component (BitVec 512) (BitVec 256) := @tophalf 512
+def top_128    : Component (BitVec 256) (BitVec 128) := @tophalf 256
+def top_64     : Component (BitVec 128) (BitVec 64)  := @tophalf 128
+def top_32     : Component (BitVec 64) (BitVec 32)   := @tophalf 64
+def top_16     : Component (BitVec 32) (BitVec 16)   := @tophalf 32
 def top_8      : Component (BitVec 16) (BitVec 8)    := @tophalf 16
 
 /-
@@ -72,6 +73,9 @@ def zerotop_64 : Component (BitVec 128) (BitVec 64) :=
 
 def zerotop_32 : Component (BitVec 64) (BitVec 32) :=
   Component.through (BitVec.truncate 32) (BitVec.truncate 64)
+
+def zerotop_16 : Component (BitVec 32) (BitVec 16) :=
+  Component.through (BitVec.truncate 16) (BitVec.truncate 32)
 
 def zerotop_8 : Component (BitVec 16) (BitVec 8) :=
   Component.through (BitVec.truncate 8) (BitVec.truncate 16)
