BignumTest/Component.lean
@@ -5,8 +5,9 @@ Author: Guilherme Lima
 -/
 
 import Bignum.Component.Basic
-
 open Bignum
+
+/-! # Unit tests for components -/
 
 structure A where
   x : Nat
@@ -21,18 +22,56 @@ def Y := Component.mk (λ a : A ↦ a.y) (λ y a ↦ {a with y := y})
 def F := Component.mk (λ b : B ↦ b.f) (λ f b ↦ {b with f := f})
 def Z := Component.mk (λ b : B ↦ b.z) (λ z b ↦ {b with z := z})
 
-#check (X : Component A Nat)
-#check (Y : Component A Bool)
-#check (F : Component B A)
-#check (Z : Component B Nat)
-#check (F :> X : Component B Nat)
-#check (F :> Y : Component B Bool)
+/-- info: X : Component A Nat     -/  #guard_msgs in #check X
+/-- info: Y : Component A Bool    -/  #guard_msgs in #check Y
+/-- info: F : Component B A       -/  #guard_msgs in #check F
+/-- info: Z : Component B Nat     -/  #guard_msgs in #check Z
+/-- info: F:>X : Component B Nat  -/  #guard_msgs in #check F:>X
+/-- info: F:>Y : Component B Bool -/  #guard_msgs in #check F:>Y
 
 def aa : A := ⟨1, false⟩
 def bb : B := ⟨aa, 2⟩
-
 example : X.read aa = aa.x := by rfl
 example : Y.read aa = aa.y := by rfl
 example : X.write 44 aa = ⟨44, false⟩ := by rfl
 example : (F :> X).read bb = 1 := by rfl
 example : (F :> X).write 99 bb = {f := {x := 99, y := false}, z := 2} := by rfl
+
+/-! ## entirety -/
+
+example : (X :> .entirety).read aa = aa.x := by rfl
+example : (.entirety :> X).read aa = aa.x := by rfl
+example : ((X :> .entirety).write 42) aa = {aa with x := 42} := by rfl
+example : ((.entirety :> X).write 42) aa = {aa with x := 42} := by rfl
+
+/-! ## rvalue -/
+
+example : (.rvalue 42 : Component Bool Nat).read true = 42 := by rfl
+example : ((.rvalue 42 : Component Bool Nat).write 33 false) = false := by rfl
+
+/-! ## element -/
+
+structure C where
+  g : Nat → Nat
+
+def G := Component.mk (λ c : C ↦ c.g) (λ g c ↦ {c with g := g})
+def G13 := (G :> .element 13)
+def cc : C := ⟨λ _ ↦ 0⟩
+
+example : G.read cc 42 = 0 := by rfl
+example : G13.read cc = 0 := by rfl
+example :  G13.read (G13.write 11 cc) = 11 := by rfl
+
+/-! ## through -/
+
+def Xr := X :> .through Nat.succ id
+def Xw := X :> .through id Nat.pred
+
+example : X.read aa = 1 := by rfl
+example : Xr.read aa = 2 := by rfl
+example : Xr.read (Xr.write 8 aa) = 9 := by rfl
+
+example : X.write 2 aa = {aa with x := 2} := by rfl
+example : (Xw.write 8 aa) = {aa with x := 7} := by rfl
+example : X.read (Xw.write 8 aa) = 7 := by rfl
+example : Xr.read (Xw.write 8 aa) = 8 := by rfl
