BignumTest/ComponentExtra.lean
@@ -5,48 +5,97 @@ Author: Guilherme Lima
 -/
 
 import Bignum.Component.Extra
+open Bignum.Component
 
-open Bignum
+set_option exponentiation.threshold 512
 
--- bitelement
+/-! # Unit test for extra components -/
 
-namespace bitelementNS
+def f512 : BitVec 512 := .allOnes 512
+def f256 : BitVec 256 := .allOnes 256
+def f128 : BitVec 128 := .allOnes 128
+def f64  : BitVec 64  := .allOnes 64
+def f32  : BitVec 32  := .allOnes 32
+def f16  : BitVec 16  := .allOnes 16
+def f8   : BitVec 8   := .allOnes 8
+
+def z512 : BitVec 512 := 0
+def z256 : BitVec 256 := 0
+def z128 : BitVec 128 := 0
+def z64  : BitVec 64  := 0
+def z32  : BitVec 32  := 0
+def z16  : BitVec 16  := 0
+def z8   : BitVec 8   := 0
+
+/-! ## bitelement -/
+
+namespace bitelement_NS
 def bv : BitVec 8 := 0b01001011#8
-example : (Component.bitelement 0).read bv = true := by rfl
-example : (Component.bitelement 1).read bv = true := by rfl
-example : (Component.bitelement 2).read bv = false := by rfl
-example : (Component.bitelement 3).read bv = true := by rfl
-example : (Component.bitelement 3).write false bv = 0b01000011#8 := by rfl
-namespace bitelementNS
+example : (bitelement 0).read bv = true := by rfl
+example : (bitelement 1).read bv = true := by rfl
+example : (bitelement 2).read bv = false := by rfl
+example : (bitelement 3).read bv = true := by rfl
+example : (bitelement 3).write false bv = 0b01000011#8 := by rfl
+namespace bitelement_NS
 
--- subword
+/-! ## subword, bottomhalf, tophalf -/
 
-namespace subwordNS
+namespace subword_NS
 def bv : BitVec 8 := 0b01001011#8
-example : (Component.subword 0 3).read bv = 0b11#3 := by rfl
-example : (Component.subword 4 1).read bv = 0#1 := by rfl
-example : (Component.subword 0 0).read bv = 0#0 := by rfl
-example : (Component.subword 6 3).read bv = 1#3 := by rfl
-example : (Component.subword 7 3).read bv = 0#3 := by rfl
-example : (Component.subword 100 2).read bv = 0#2 := by rfl
-example : (Component.subword 0 3).write 0 bv = 0b01001000#8 := by rfl
-example : (Component.subword 1 3).write 0b101 bv = 0b01001011#8 := by rfl
-example : (Component.subword 6 4).write 0xf bv = 0b11001011#8 := by rfl
-example : Component.bottomhalf.read bv = 0b1011#4 := by rfl
-example : Component.bottomhalf.read 0b11#2 = 0b1#1 := by rfl
-example : Component.bottomhalf.read 0b11#0 = 0b1#0 := by rfl
-example : Component.bottomhalf.write 0xf bv = 0b01001111#8 := by rfl
-example : Component.bottomhalf.write 0xf 0#2 = 1#2 := by rfl
-example : Component.bottomhalf.write 0xf 0#0 = 0#0 := by rfl
-example : Component.tophalf.read bv = 0b0100#4 := by rfl
-example : Component.tophalf.read 0b11#2 = 0b1#1 := by rfl
-example : Component.tophalf.read 0b11#0 = 0b1#0 := by rfl
-example : Component.tophalf.write 0xf bv = 0b11111011#8 := by rfl
-example : Component.tophalf.write 0xf 0#2 = 2#2 := by rfl
-example : Component.tophalf.write 0xf 0#0 = 0#0 := by rfl
-example : Component.tophalf.write 0x0 111#3 = 0b001#3 := by rfl
-example : Component.zerotop_32.read (BitVec.allOnes 64)
-          = BitVec.allOnes 32 := by rfl
-example : Component.zerotop_32.write (BitVec.allOnes 32) (BitVec.allOnes 64)
-          = 0#32 ++ (BitVec.allOnes 32) := by rfl
-end subwordNS
+example : (subword 0 3).read bv = 0b11#3 := by rfl
+example : (subword 4 1).read bv = 0#1 := by rfl
+example : (subword 0 0).read bv = 0#0 := by rfl
+example : (subword 6 3).read bv = 1#3 := by rfl
+example : (subword 7 3).read bv = 0#3 := by rfl
+example : (subword 100 2).read bv = 0#2 := by rfl
+example : (subword 0 3).write 0 bv = 0b01001000#8 := by rfl
+example : (subword 1 3).write 0b101 bv = 0b01001011#8 := by rfl
+example : (subword 6 4).write 0xf bv = 0b11001011#8 := by rfl
+example : bottomhalf.read bv = 0b1011#4 := by rfl
+example : bottomhalf.read 0b11#2 = 0b1#1 := by rfl
+example : bottomhalf.read 0b11#0 = 0b1#0 := by rfl
+example : bottomhalf.write 0xf bv = 0b01001111#8 := by rfl
+example : bottomhalf.write 0xf 0#2 = 1#2 := by rfl
+example : bottomhalf.write 0xf 0#0 = 0#0 := by rfl
+example : tophalf.read bv = 0b0100#4 := by rfl
+example : tophalf.read 0b11#2 = 0b1#1 := by rfl
+example : tophalf.read 0b11#0 = 0b1#0 := by rfl
+example : tophalf.write 0xf bv = 0b11111011#8 := by rfl
+example : tophalf.write 0xf 0#2 = 2#2 := by rfl
+example : tophalf.write 0xf 0#0 = 0#0 := by rfl
+example : tophalf.write 0x0 111#3 = 0b001#3 := by rfl
+end subword_NS
+
+/-! ## bottom_*, top_* -/
+
+namespace bottom_top_NS
+example : bottom_256.read f512 = f256 := by rfl
+example : bottom_128.read f256 = f128 := by rfl
+example : bottom_64.read f128 = f64 := by rfl
+example : bottom_32.read f64 = f32 := by rfl
+example : bottom_16.read f32 = f16 := by rfl
+example : bottom_8.read f16 = f8 := by rfl
+example : top_256.read f512 = f256 := by rfl
+example : top_128.read f256 = f128 := by rfl
+example : top_64.read f128 = f64 := by rfl
+example : top_32.read f64 = f32 := by rfl
+example : top_16.read f32 = f16 := by rfl
+example : top_8.read f16 = f8 := by rfl
+end bottom_top_NS
+
+/-! ## zerotop_* -/
+
+namespace zerotop_NS
+example : zerotop_256.read f512 = f256 := by rfl
+example : zerotop_256.write f256 f512 = z256 ++ f256 := by rfl
+example : zerotop_128.read f256 = f128 := by rfl
+example : zerotop_128.write f128 f256 = z128 ++ f128 := by rfl
+example : zerotop_64.read f128 = f64 := by rfl
+example : zerotop_64.write f64 f128 = z64 ++ f64 := by rfl
+example : zerotop_32.read f64 = f32 := by rfl
+example : zerotop_32.write f32 f64 = z32 ++ f32 := by rfl
+example : zerotop_16.read f32 = f16 := by rfl
+example : zerotop_16.write f16 f32 = z16 ++ f16 := by rfl
+example : zerotop_8.read f16 = f8 := by rfl
+example : zerotop_8.write f8 f16 = z8 ++ f8 := by rfl
+end zerotop_NS
