BignumTest/ArmRev/State.lean
@@ -5,234 +5,364 @@ Author: Guilherme Lima
 -/
 
 import Bignum.ArmRev
+open Bignum.ArmRev.State
 
-open Bignum.ArmRev
+/-! # Unit tests for ARM state -/
 
-open State
+def S₀ := allZeros
+def S₁ := allOnes
 
--- allZeros
+/-! ## allZeros -/
 
-example : NF.read allZeros = false := by rfl
-example : ZF.read allZeros = false := by rfl
-example : CF.read allZeros = false := by rfl
-example : VF.read allZeros = false := by rfl
+example : allZeros._PC               = 0  := by rfl
+example : allZeros._registers 42     = 0  := by rfl
+example : allZeros._simdregisters 42 = 0  := by rfl
+example : allZeros._flags            = 0  := by rfl
+example : allZeros._memory 42        = 0  := by rfl
+example : allZeros._events           = [] := by rfl
 
-example : NF.read (NF.write true allZeros) = true := by rfl
-example : NF.read (ZF.write true allZeros) = false := by rfl
+/-! ## allOnes -/
 
-example : (NF.write true allZeros)._flags = 0b1000 := by rfl
-example : (ZF.write true allZeros)._flags = 0b0100 := by rfl
-example : (CF.write true allZeros)._flags = 0b0010 := by rfl
-example : (VF.write true allZeros)._flags = 0b0001 := by rfl
+example : allOnes._PC               = .allOnes 64  := by rfl
+example : allOnes._registers 42     = .allOnes 64  := by rfl
+example : allOnes._simdregisters 42 = .allOnes 128 := by rfl
+example : allOnes._flags            = .allOnes 4   := by rfl
+example : allOnes._memory 42        = .allOnes 8   := by rfl
+example : allOnes._events           = []           := by rfl
 
-example : XZR.read allZeros = 0#64 := by rfl
-example : XZR.read (XZR.write 1 allZeros) = 0#64 := by rfl
-example : WZR.read allZeros = 0#32 := by rfl
-example : WZR.read (WZR.write 1 allZeros) = 0#32 := by rfl
+/-! ## State components -/
 
-example : X0.read allZeros = 0#64 := by rfl
-example : X1.read allZeros = 0#64 := by rfl
-example : X2.read allZeros = 0#64 := by rfl
-example : X3.read allZeros = 0#64 := by rfl
-example : X4.read allZeros = 0#64 := by rfl
-example : X5.read allZeros = 0#64 := by rfl
-example : X6.read allZeros = 0#64 := by rfl
-example : X7.read allZeros = 0#64 := by rfl
-example : X8.read allZeros = 0#64 := by rfl
-example : X9.read allZeros = 0#64 := by rfl
-example : X10.read allZeros = 0#64 := by rfl
-example : X11.read allZeros = 0#64 := by rfl
-example : X12.read allZeros = 0#64 := by rfl
-example : X13.read allZeros = 0#64 := by rfl
-example : X14.read allZeros = 0#64 := by rfl
-example : X15.read allZeros = 0#64 := by rfl
-example : X16.read allZeros = 0#64 := by rfl
-example : X17.read allZeros = 0#64 := by rfl
-example : X18.read allZeros = 0#64 := by rfl
-example : X19.read allZeros = 0#64 := by rfl
-example : X20.read allZeros = 0#64 := by rfl
-example : X21.read allZeros = 0#64 := by rfl
-example : X22.read allZeros = 0#64 := by rfl
-example : X23.read allZeros = 0#64 := by rfl
-example : X24.read allZeros = 0#64 := by rfl
-example : X25.read allZeros = 0#64 := by rfl
-example : X26.read allZeros = 0#64 := by rfl
-example : X27.read allZeros = 0#64 := by rfl
-example : X28.read allZeros = 0#64 := by rfl
-example : X29.read allZeros = 0#64 := by rfl
-example : X30.read allZeros = 0#64 := by rfl
-example : SP.read allZeros = 0#64 := by rfl
+example : PC.read S₀            = S₀._PC            := by rfl
+example : PC.read S₁            = S₁._PC            := by rfl
+example : registers.read S₀     = S₀._registers     := by rfl
+example : registers.read S₁     = S₁._registers     := by rfl
+example : simdregisters.read S₀ = S₀._simdregisters := by rfl
+example : simdregisters.read S₁ = S₁._simdregisters := by rfl
+example : flags.read S₀         = S₀._flags         := by rfl
+example : flags.read S₁         = S₁._flags         := by rfl
+example : memory.read S₀        = S₀._memory        := by rfl
+example : memory.read S₁        = S₁._memory        := by rfl
+example : events.read S₀        = S₀._events        := by rfl
+example : events.read S₁        = S₁._events        := by rfl
 
-example : (X0.write 0xff allZeros)._registers 0 = 0xff := by rfl
-example : (X1.write 0xff allZeros)._registers 1 = 0xff := by rfl
-example : (X2.write 0xff allZeros)._registers 2 = 0xff := by rfl
-example : (X3.write 0xff allZeros)._registers 3 = 0xff := by rfl
-example : (X4.write 0xff allZeros)._registers 4 = 0xff := by rfl
-example : (X5.write 0xff allZeros)._registers 5 = 0xff := by rfl
-example : (X6.write 0xff allZeros)._registers 6 = 0xff := by rfl
-example : (X7.write 0xff allZeros)._registers 7 = 0xff := by rfl
-example : (X8.write 0xff allZeros)._registers 8 = 0xff := by rfl
-example : (X9.write 0xff allZeros)._registers 9 = 0xff := by rfl
-example : (X10.write 0xff allZeros)._registers 10 = 0xff := by rfl
-example : (X11.write 0xff allZeros)._registers 11 = 0xff := by rfl
-example : (X12.write 0xff allZeros)._registers 12 = 0xff := by rfl
-example : (X13.write 0xff allZeros)._registers 13 = 0xff := by rfl
-example : (X14.write 0xff allZeros)._registers 14 = 0xff := by rfl
-example : (X15.write 0xff allZeros)._registers 15 = 0xff := by rfl
-example : (X16.write 0xff allZeros)._registers 16 = 0xff := by rfl
-example : (X17.write 0xff allZeros)._registers 17 = 0xff := by rfl
-example : (X18.write 0xff allZeros)._registers 18 = 0xff := by rfl
-example : (X19.write 0xff allZeros)._registers 19 = 0xff := by rfl
-example : (X20.write 0xff allZeros)._registers 20 = 0xff := by rfl
-example : (X21.write 0xff allZeros)._registers 21 = 0xff := by rfl
-example : (X22.write 0xff allZeros)._registers 22 = 0xff := by rfl
-example : (X23.write 0xff allZeros)._registers 23 = 0xff := by rfl
-example : (X24.write 0xff allZeros)._registers 24 = 0xff := by rfl
-example : (X25.write 0xff allZeros)._registers 25 = 0xff := by rfl
-example : (X26.write 0xff allZeros)._registers 26 = 0xff := by rfl
-example : (X27.write 0xff allZeros)._registers 27 = 0xff := by rfl
-example : (X28.write 0xff allZeros)._registers 28 = 0xff := by rfl
-example : (X29.write 0xff allZeros)._registers 29 = 0xff := by rfl
-example : (X30.write 0xff allZeros)._registers 30 = 0xff := by rfl
-example : (SP.write 0xff allZeros)._registers 31 = 0xff := by rfl
-example : ((XREG 31).write 0xff allZeros)._registers 31 = 0x0 := by rfl
+example : PC.read (PC.write 1 S₀) = 1 := by rfl
+example : flags.read (PC.write 1 S₀) = 0 := by rfl
+example : PC.read (PC.write 1 S₁) = 1 := by rfl
+example : flags.read (PC.write 1 S₁) = .allOnes 4 := by rfl
 
-example : W0.read allZeros = 0#32 := by rfl
-example : W1.read allZeros = 0#32 := by rfl
-example : W2.read allZeros = 0#32 := by rfl
-example : W3.read allZeros = 0#32 := by rfl
-example : W4.read allZeros = 0#32 := by rfl
-example : W5.read allZeros = 0#32 := by rfl
-example : W6.read allZeros = 0#32 := by rfl
-example : W7.read allZeros = 0#32 := by rfl
-example : W8.read allZeros = 0#32 := by rfl
-example : W9.read allZeros = 0#32 := by rfl
-example : W10.read allZeros = 0#32 := by rfl
-example : W11.read allZeros = 0#32 := by rfl
-example : W12.read allZeros = 0#32 := by rfl
-example : W13.read allZeros = 0#32 := by rfl
-example : W14.read allZeros = 0#32 := by rfl
-example : W15.read allZeros = 0#32 := by rfl
-example : W16.read allZeros = 0#32 := by rfl
-example : W17.read allZeros = 0#32 := by rfl
-example : W18.read allZeros = 0#32 := by rfl
-example : W19.read allZeros = 0#32 := by rfl
-example : W20.read allZeros = 0#32 := by rfl
-example : W21.read allZeros = 0#32 := by rfl
-example : W22.read allZeros = 0#32 := by rfl
-example : W23.read allZeros = 0#32 := by rfl
-example : W24.read allZeros = 0#32 := by rfl
-example : W25.read allZeros = 0#32 := by rfl
-example : W26.read allZeros = 0#32 := by rfl
-example : W27.read allZeros = 0#32 := by rfl
-example : W28.read allZeros = 0#32 := by rfl
-example : W29.read allZeros = 0#32 := by rfl
-example : W30.read allZeros = 0#32 := by rfl
-example : WSP.read allZeros = 0#32 := by rfl
+/-! ## Condition flags -/
 
-example : (W0.write 0xff allZeros)._registers 0 = 0xff := by rfl
-example : (W1.write 0xff allZeros)._registers 1 = 0xff := by rfl
-example : (W2.write 0xff allZeros)._registers 2 = 0xff := by rfl
-example : (W3.write 0xff allZeros)._registers 3 = 0xff := by rfl
-example : (W4.write 0xff allZeros)._registers 4 = 0xff := by rfl
-example : (W5.write 0xff allZeros)._registers 5 = 0xff := by rfl
-example : (W6.write 0xff allZeros)._registers 6 = 0xff := by rfl
-example : (W7.write 0xff allZeros)._registers 7 = 0xff := by rfl
-example : (W8.write 0xff allZeros)._registers 8 = 0xff := by rfl
-example : (W9.write 0xff allZeros)._registers 9 = 0xff := by rfl
-example : (W10.write 0xff allZeros)._registers 10 = 0xff := by rfl
-example : (W11.write 0xff allZeros)._registers 11 = 0xff := by rfl
-example : (W12.write 0xff allZeros)._registers 12 = 0xff := by rfl
-example : (W13.write 0xff allZeros)._registers 13 = 0xff := by rfl
-example : (W14.write 0xff allZeros)._registers 14 = 0xff := by rfl
-example : (W15.write 0xff allZeros)._registers 15 = 0xff := by rfl
-example : (W16.write 0xff allZeros)._registers 16 = 0xff := by rfl
-example : (W17.write 0xff allZeros)._registers 17 = 0xff := by rfl
-example : (W18.write 0xff allZeros)._registers 18 = 0xff := by rfl
-example : (W19.write 0xff allZeros)._registers 19 = 0xff := by rfl
-example : (W20.write 0xff allZeros)._registers 20 = 0xff := by rfl
-example : (W21.write 0xff allZeros)._registers 21 = 0xff := by rfl
-example : (W22.write 0xff allZeros)._registers 22 = 0xff := by rfl
-example : (W23.write 0xff allZeros)._registers 23 = 0xff := by rfl
-example : (W24.write 0xff allZeros)._registers 24 = 0xff := by rfl
-example : (W25.write 0xff allZeros)._registers 25 = 0xff := by rfl
-example : (W26.write 0xff allZeros)._registers 26 = 0xff := by rfl
-example : (W27.write 0xff allZeros)._registers 27 = 0xff := by rfl
-example : (W28.write 0xff allZeros)._registers 28 = 0xff := by rfl
-example : (W29.write 0xff allZeros)._registers 29 = 0xff := by rfl
-example : (W30.write 0xff allZeros)._registers 30 = 0xff := by rfl
-example : (WSP.write 0xff allZeros)._registers 31 = 0xff := by rfl
-example : ((WREG 31).write 0xff allZeros)._registers 31 = 0x0 := by rfl
+example : NF.read S₀ = false := by rfl
+example : ZF.read S₀ = false := by rfl
+example : CF.read S₀ = false := by rfl
+example : VF.read S₀ = false := by rfl
 
--- allOnes
+example : NF.read S₁ = true := by rfl
+example : ZF.read S₁ = true := by rfl
+example : CF.read S₁ = true := by rfl
+example : VF.read S₁ = true := by rfl
 
-example : NF.read allOnes = true := by rfl
-example : ZF.read allOnes = true := by rfl
-example : CF.read allOnes = true := by rfl
-example : VF.read allOnes = true := by rfl
+example : NF.read (NF.write true S₀) = true := by rfl
+example : NF.read (ZF.write true S₀) = false := by rfl
+example : NF.read (NF.write false S₁) = false := by rfl
+example : NF.read (ZF.write false S₁) = true := by rfl
 
-example : XZR.read allOnes = 0#64 := by rfl
--- example : State.allOnes.X0 = 0xffffffffffffffff#64 := by rfl
--- example : State.allOnes.X1 = 0xffffffffffffffff#64 := by rfl
--- example : State.allOnes.X2 = 0xffffffffffffffff#64 := by rfl
--- example : State.allOnes.X3 = 0xffffffffffffffff#64 := by rfl
--- example : State.allOnes.X4 = 0xffffffffffffffff#64 := by rfl
--- example : State.allOnes.X5 = 0xffffffffffffffff#64 := by rfl
--- example : State.allOnes.X6 = 0xffffffffffffffff#64 := by rfl
--- example : State.allOnes.X7 = 0xffffffffffffffff#64 := by rfl
--- example : State.allOnes.X8 = 0xffffffffffffffff#64 := by rfl
--- example : State.allOnes.X9 = 0xffffffffffffffff#64 := by rfl
--- example : State.allOnes.X10 = 0xffffffffffffffff#64 := by rfl
--- example : State.allOnes.X11 = 0xffffffffffffffff#64 := by rfl
--- example : State.allOnes.X12 = 0xffffffffffffffff#64 := by rfl
--- example : State.allOnes.X13 = 0xffffffffffffffff#64 := by rfl
--- example : State.allOnes.X14 = 0xffffffffffffffff#64 := by rfl
--- example : State.allOnes.X15 = 0xffffffffffffffff#64 := by rfl
--- example : State.allOnes.X16 = 0xffffffffffffffff#64 := by rfl
--- example : State.allOnes.X17 = 0xffffffffffffffff#64 := by rfl
--- example : State.allOnes.X18 = 0xffffffffffffffff#64 := by rfl
--- example : State.allOnes.X19 = 0xffffffffffffffff#64 := by rfl
--- example : State.allOnes.X20 = 0xffffffffffffffff#64 := by rfl
--- example : State.allOnes.X21 = 0xffffffffffffffff#64 := by rfl
--- example : State.allOnes.X22 = 0xffffffffffffffff#64 := by rfl
--- example : State.allOnes.X23 = 0xffffffffffffffff#64 := by rfl
--- example : State.allOnes.X24 = 0xffffffffffffffff#64 := by rfl
--- example : State.allOnes.X25 = 0xffffffffffffffff#64 := by rfl
--- example : State.allOnes.X26 = 0xffffffffffffffff#64 := by rfl
--- example : State.allOnes.X27 = 0xffffffffffffffff#64 := by rfl
--- example : State.allOnes.X28 = 0xffffffffffffffff#64 := by rfl
--- example : State.allOnes.X29 = 0xffffffffffffffff#64 := by rfl
--- example : State.allOnes.X30 = 0xffffffffffffffff#64 := by rfl
--- example : State.allOnes.SP = 0xffffffffffffffff#64 := by rfl
--- example : State.allOnes.W0 = 0xffffffff#32 := by rfl
--- example : State.allOnes.W1 = 0xffffffff#32 := by rfl
--- example : State.allOnes.W2 = 0xffffffff#32 := by rfl
--- example : State.allOnes.W3 = 0xffffffff#32 := by rfl
--- example : State.allOnes.W4 = 0xffffffff#32 := by rfl
--- example : State.allOnes.W5 = 0xffffffff#32 := by rfl
--- example : State.allOnes.W6 = 0xffffffff#32 := by rfl
--- example : State.allOnes.W7 = 0xffffffff#32 := by rfl
--- example : State.allOnes.W8 = 0xffffffff#32 := by rfl
--- example : State.allOnes.W9 = 0xffffffff#32 := by rfl
--- example : State.allOnes.W10 = 0xffffffff#32 := by rfl
--- example : State.allOnes.W11 = 0xffffffff#32 := by rfl
--- example : State.allOnes.W12 = 0xffffffff#32 := by rfl
--- example : State.allOnes.W13 = 0xffffffff#32 := by rfl
--- example : State.allOnes.W14 = 0xffffffff#32 := by rfl
--- example : State.allOnes.W15 = 0xffffffff#32 := by rfl
--- example : State.allOnes.W16 = 0xffffffff#32 := by rfl
--- example : State.allOnes.W17 = 0xffffffff#32 := by rfl
--- example : State.allOnes.W18 = 0xffffffff#32 := by rfl
--- example : State.allOnes.W19 = 0xffffffff#32 := by rfl
--- example : State.allOnes.W20 = 0xffffffff#32 := by rfl
--- example : State.allOnes.W21 = 0xffffffff#32 := by rfl
--- example : State.allOnes.W22 = 0xffffffff#32 := by rfl
--- example : State.allOnes.W23 = 0xffffffff#32 := by rfl
--- example : State.allOnes.W24 = 0xffffffff#32 := by rfl
--- example : State.allOnes.W25 = 0xffffffff#32 := by rfl
--- example : State.allOnes.W26 = 0xffffffff#32 := by rfl
--- example : State.allOnes.W27 = 0xffffffff#32 := by rfl
--- example : State.allOnes.W28 = 0xffffffff#32 := by rfl
--- example : State.allOnes.W29 = 0xffffffff#32 := by rfl
--- example : State.allOnes.W30 = 0xffffffff#32 := by rfl
--- example : State.allOnes.WSP = 0xffffffff#32 := by rfl
+example : (NF.write true S₀)._flags = 0b1000 := by rfl
+example : (ZF.write true S₀)._flags = 0b0100 := by rfl
+example : (CF.write true S₀)._flags = 0b0010 := by rfl
+example : (VF.write true S₀)._flags = 0b0001 := by rfl
+
+example : (NF.write false S₁)._flags = 0b0111 := by rfl
+example : (ZF.write false S₁)._flags = 0b1011 := by rfl
+example : (CF.write false S₁)._flags = 0b1101 := by rfl
+example : (VF.write false S₁)._flags = 0b1110 := by rfl
+
+/-! ## Zero registers -/
+
+example : XZR.read S₀ = 0#64 := by rfl
+example : XZR.read S₁ = 0#64 := by rfl
+example : XZR.read (XZR.write 1 S₀) = 0#64 := by rfl
+example : XZR.read (XZR.write 1 S₁) = 0#64 := by rfl
+
+example : WZR.read S₀ = 0#32 := by rfl
+example : WZR.read S₁ = 0#32 := by rfl
+example : WZR.read (WZR.write 1 S₀) = 0#32 := by rfl
+example : WZR.read (WZR.write 1 S₁) = 0#32 := by rfl
+
+/-! ## Main registers -/
+
+example : X0.read S₀  = 0#64 := by rfl
+example : X1.read S₀  = 0#64 := by rfl
+example : X2.read S₀  = 0#64 := by rfl
+example : X3.read S₀  = 0#64 := by rfl
+example : X4.read S₀  = 0#64 := by rfl
+example : X5.read S₀  = 0#64 := by rfl
+example : X6.read S₀  = 0#64 := by rfl
+example : X7.read S₀  = 0#64 := by rfl
+example : X8.read S₀  = 0#64 := by rfl
+example : X9.read S₀  = 0#64 := by rfl
+example : X10.read S₀ = 0#64 := by rfl
+example : X11.read S₀ = 0#64 := by rfl
+example : X12.read S₀ = 0#64 := by rfl
+example : X13.read S₀ = 0#64 := by rfl
+example : X14.read S₀ = 0#64 := by rfl
+example : X15.read S₀ = 0#64 := by rfl
+example : X16.read S₀ = 0#64 := by rfl
+example : X17.read S₀ = 0#64 := by rfl
+example : X18.read S₀ = 0#64 := by rfl
+example : X19.read S₀ = 0#64 := by rfl
+example : X20.read S₀ = 0#64 := by rfl
+example : X21.read S₀ = 0#64 := by rfl
+example : X22.read S₀ = 0#64 := by rfl
+example : X23.read S₀ = 0#64 := by rfl
+example : X24.read S₀ = 0#64 := by rfl
+example : X25.read S₀ = 0#64 := by rfl
+example : X26.read S₀ = 0#64 := by rfl
+example : X27.read S₀ = 0#64 := by rfl
+example : X28.read S₀ = 0#64 := by rfl
+example : X29.read S₀ = 0#64 := by rfl
+example : X30.read S₀ = 0#64 := by rfl
+example : SP.read S₀  = 0#64 := by rfl
+
+example : X0.read S₁  = .allOnes 64 := by rfl
+example : X1.read S₁  = .allOnes 64 := by rfl
+example : X2.read S₁  = .allOnes 64 := by rfl
+example : X3.read S₁  = .allOnes 64 := by rfl
+example : X4.read S₁  = .allOnes 64 := by rfl
+example : X5.read S₁  = .allOnes 64 := by rfl
+example : X6.read S₁  = .allOnes 64 := by rfl
+example : X7.read S₁  = .allOnes 64 := by rfl
+example : X8.read S₁  = .allOnes 64 := by rfl
+example : X9.read S₁  = .allOnes 64 := by rfl
+example : X10.read S₁ = .allOnes 64 := by rfl
+example : X11.read S₁ = .allOnes 64 := by rfl
+example : X12.read S₁ = .allOnes 64 := by rfl
+example : X13.read S₁ = .allOnes 64 := by rfl
+example : X14.read S₁ = .allOnes 64 := by rfl
+example : X15.read S₁ = .allOnes 64 := by rfl
+example : X16.read S₁ = .allOnes 64 := by rfl
+example : X17.read S₁ = .allOnes 64 := by rfl
+example : X18.read S₁ = .allOnes 64 := by rfl
+example : X19.read S₁ = .allOnes 64 := by rfl
+example : X20.read S₁ = .allOnes 64 := by rfl
+example : X21.read S₁ = .allOnes 64 := by rfl
+example : X22.read S₁ = .allOnes 64 := by rfl
+example : X23.read S₁ = .allOnes 64 := by rfl
+example : X24.read S₁ = .allOnes 64 := by rfl
+example : X25.read S₁ = .allOnes 64 := by rfl
+example : X26.read S₁ = .allOnes 64 := by rfl
+example : X27.read S₁ = .allOnes 64 := by rfl
+example : X28.read S₁ = .allOnes 64 := by rfl
+example : X29.read S₁ = .allOnes 64 := by rfl
+example : X30.read S₁ = .allOnes 64 := by rfl
+example : SP.read S₁  = .allOnes 64 := by rfl
+
+example : (X0.write 1 S₀)._registers 0 = 1 := by rfl
+example : (X1.write 1 S₀)._registers 1 = 1 := by rfl
+example : (X2.write 1 S₀)._registers 2 = 1 := by rfl
+example : (X3.write 1 S₀)._registers 3 = 1 := by rfl
+example : (X4.write 1 S₀)._registers 4 = 1 := by rfl
+example : (X5.write 1 S₀)._registers 5 = 1 := by rfl
+example : (X6.write 1 S₀)._registers 6 = 1 := by rfl
+example : (X7.write 1 S₀)._registers 7 = 1 := by rfl
+example : (X8.write 1 S₀)._registers 8 = 1 := by rfl
+example : (X9.write 1 S₀)._registers 9 = 1 := by rfl
+example : (X10.write 1 S₀)._registers 10 = 1 := by rfl
+example : (X11.write 1 S₀)._registers 11 = 1 := by rfl
+example : (X12.write 1 S₀)._registers 12 = 1 := by rfl
+example : (X13.write 1 S₀)._registers 13 = 1 := by rfl
+example : (X14.write 1 S₀)._registers 14 = 1 := by rfl
+example : (X15.write 1 S₀)._registers 15 = 1 := by rfl
+example : (X16.write 1 S₀)._registers 16 = 1 := by rfl
+example : (X17.write 1 S₀)._registers 17 = 1 := by rfl
+example : (X18.write 1 S₀)._registers 18 = 1 := by rfl
+example : (X19.write 1 S₀)._registers 19 = 1 := by rfl
+example : (X20.write 1 S₀)._registers 20 = 1 := by rfl
+example : (X21.write 1 S₀)._registers 21 = 1 := by rfl
+example : (X22.write 1 S₀)._registers 22 = 1 := by rfl
+example : (X23.write 1 S₀)._registers 23 = 1 := by rfl
+example : (X24.write 1 S₀)._registers 24 = 1 := by rfl
+example : (X25.write 1 S₀)._registers 25 = 1 := by rfl
+example : (X26.write 1 S₀)._registers 26 = 1 := by rfl
+example : (X27.write 1 S₀)._registers 27 = 1 := by rfl
+example : (X28.write 1 S₀)._registers 28 = 1 := by rfl
+example : (X29.write 1 S₀)._registers 29 = 1 := by rfl
+example : (X30.write 1 S₀)._registers 30 = 1 := by rfl
+example : (SP.write 1 S₀)._registers 31 = 1 := by rfl
+
+example : (X0.write 0 S₁)._registers 0 = 0 := by rfl
+example : (X1.write 0 S₁)._registers 1 = 0 := by rfl
+example : (X2.write 0 S₁)._registers 2 = 0 := by rfl
+example : (X3.write 0 S₁)._registers 3 = 0 := by rfl
+example : (X4.write 0 S₁)._registers 4 = 0 := by rfl
+example : (X5.write 0 S₁)._registers 5 = 0 := by rfl
+example : (X6.write 0 S₁)._registers 6 = 0 := by rfl
+example : (X7.write 0 S₁)._registers 7 = 0 := by rfl
+example : (X8.write 0 S₁)._registers 8 = 0 := by rfl
+example : (X9.write 0 S₁)._registers 9 = 0 := by rfl
+example : (X10.write 0 S₁)._registers 10 = 0 := by rfl
+example : (X11.write 0 S₁)._registers 11 = 0 := by rfl
+example : (X12.write 0 S₁)._registers 12 = 0 := by rfl
+example : (X13.write 0 S₁)._registers 13 = 0 := by rfl
+example : (X14.write 0 S₁)._registers 14 = 0 := by rfl
+example : (X15.write 0 S₁)._registers 15 = 0 := by rfl
+example : (X16.write 0 S₁)._registers 16 = 0 := by rfl
+example : (X17.write 0 S₁)._registers 17 = 0 := by rfl
+example : (X18.write 0 S₁)._registers 18 = 0 := by rfl
+example : (X19.write 0 S₁)._registers 19 = 0 := by rfl
+example : (X20.write 0 S₁)._registers 20 = 0 := by rfl
+example : (X21.write 0 S₁)._registers 21 = 0 := by rfl
+example : (X22.write 0 S₁)._registers 22 = 0 := by rfl
+example : (X23.write 0 S₁)._registers 23 = 0 := by rfl
+example : (X24.write 0 S₁)._registers 24 = 0 := by rfl
+example : (X25.write 0 S₁)._registers 25 = 0 := by rfl
+example : (X26.write 0 S₁)._registers 26 = 0 := by rfl
+example : (X27.write 0 S₁)._registers 27 = 0 := by rfl
+example : (X28.write 0 S₁)._registers 28 = 0 := by rfl
+example : (X29.write 0 S₁)._registers 29 = 0 := by rfl
+example : (X30.write 0 S₁)._registers 30 = 0 := by rfl
+example : (SP.write 0 S₁)._registers 31 = 0 := by rfl
+
+example : (XREG 31).read ((XREG 31).write 1 S₀) = 0 := by rfl
+example : (XREG 31).read ((XREG 31).write 8 S₁) = 0 := by rfl
+
+/-! ## 32-bit versions of the main registers -/
+
+example : W0.read S₀  = 0#32 := by rfl
+example : W1.read S₀  = 0#32 := by rfl
+example : W2.read S₀  = 0#32 := by rfl
+example : W3.read S₀  = 0#32 := by rfl
+example : W4.read S₀  = 0#32 := by rfl
+example : W5.read S₀  = 0#32 := by rfl
+example : W6.read S₀  = 0#32 := by rfl
+example : W7.read S₀  = 0#32 := by rfl
+example : W8.read S₀  = 0#32 := by rfl
+example : W9.read S₀  = 0#32 := by rfl
+example : W10.read S₀ = 0#32 := by rfl
+example : W11.read S₀ = 0#32 := by rfl
+example : W12.read S₀ = 0#32 := by rfl
+example : W13.read S₀ = 0#32 := by rfl
+example : W14.read S₀ = 0#32 := by rfl
+example : W15.read S₀ = 0#32 := by rfl
+example : W16.read S₀ = 0#32 := by rfl
+example : W17.read S₀ = 0#32 := by rfl
+example : W18.read S₀ = 0#32 := by rfl
+example : W19.read S₀ = 0#32 := by rfl
+example : W20.read S₀ = 0#32 := by rfl
+example : W21.read S₀ = 0#32 := by rfl
+example : W22.read S₀ = 0#32 := by rfl
+example : W23.read S₀ = 0#32 := by rfl
+example : W24.read S₀ = 0#32 := by rfl
+example : W25.read S₀ = 0#32 := by rfl
+example : W26.read S₀ = 0#32 := by rfl
+example : W27.read S₀ = 0#32 := by rfl
+example : W28.read S₀ = 0#32 := by rfl
+example : W29.read S₀ = 0#32 := by rfl
+example : W30.read S₀ = 0#32 := by rfl
+example : WSP.read S₀ = 0#32 := by rfl
+
+example : W0.read S₁  = .allOnes 32 := by rfl
+example : W1.read S₁  = .allOnes 32 := by rfl
+example : W2.read S₁  = .allOnes 32 := by rfl
+example : W3.read S₁  = .allOnes 32 := by rfl
+example : W4.read S₁  = .allOnes 32 := by rfl
+example : W5.read S₁  = .allOnes 32 := by rfl
+example : W6.read S₁  = .allOnes 32 := by rfl
+example : W7.read S₁  = .allOnes 32 := by rfl
+example : W8.read S₁  = .allOnes 32 := by rfl
+example : W9.read S₁  = .allOnes 32 := by rfl
+example : W10.read S₁ = .allOnes 32 := by rfl
+example : W11.read S₁ = .allOnes 32 := by rfl
+example : W12.read S₁ = .allOnes 32 := by rfl
+example : W13.read S₁ = .allOnes 32 := by rfl
+example : W14.read S₁ = .allOnes 32 := by rfl
+example : W15.read S₁ = .allOnes 32 := by rfl
+example : W16.read S₁ = .allOnes 32 := by rfl
+example : W17.read S₁ = .allOnes 32 := by rfl
+example : W18.read S₁ = .allOnes 32 := by rfl
+example : W19.read S₁ = .allOnes 32 := by rfl
+example : W20.read S₁ = .allOnes 32 := by rfl
+example : W21.read S₁ = .allOnes 32 := by rfl
+example : W22.read S₁ = .allOnes 32 := by rfl
+example : W23.read S₁ = .allOnes 32 := by rfl
+example : W24.read S₁ = .allOnes 32 := by rfl
+example : W25.read S₁ = .allOnes 32 := by rfl
+example : W26.read S₁ = .allOnes 32 := by rfl
+example : W27.read S₁ = .allOnes 32 := by rfl
+example : W28.read S₁ = .allOnes 32 := by rfl
+example : W29.read S₁ = .allOnes 32 := by rfl
+example : W30.read S₁ = .allOnes 32 := by rfl
+example : WSP.read S₁ = .allOnes 32 := by rfl
+
+example : (W0.write 1 S₀)._registers 0 = 1 := by rfl
+example : (W1.write 1 S₀)._registers 1 = 1 := by rfl
+example : (W2.write 1 S₀)._registers 2 = 1 := by rfl
+example : (W3.write 1 S₀)._registers 3 = 1 := by rfl
+example : (W4.write 1 S₀)._registers 4 = 1 := by rfl
+example : (W5.write 1 S₀)._registers 5 = 1 := by rfl
+example : (W6.write 1 S₀)._registers 6 = 1 := by rfl
+example : (W7.write 1 S₀)._registers 7 = 1 := by rfl
+example : (W8.write 1 S₀)._registers 8 = 1 := by rfl
+example : (W9.write 1 S₀)._registers 9 = 1 := by rfl
+example : (W10.write 1 S₀)._registers 10 = 1 := by rfl
+example : (W11.write 1 S₀)._registers 11 = 1 := by rfl
+example : (W12.write 1 S₀)._registers 12 = 1 := by rfl
+example : (W13.write 1 S₀)._registers 13 = 1 := by rfl
+example : (W14.write 1 S₀)._registers 14 = 1 := by rfl
+example : (W15.write 1 S₀)._registers 15 = 1 := by rfl
+example : (W16.write 1 S₀)._registers 16 = 1 := by rfl
+example : (W17.write 1 S₀)._registers 17 = 1 := by rfl
+example : (W18.write 1 S₀)._registers 18 = 1 := by rfl
+example : (W19.write 1 S₀)._registers 19 = 1 := by rfl
+example : (W20.write 1 S₀)._registers 20 = 1 := by rfl
+example : (W21.write 1 S₀)._registers 21 = 1 := by rfl
+example : (W22.write 1 S₀)._registers 22 = 1 := by rfl
+example : (W23.write 1 S₀)._registers 23 = 1 := by rfl
+example : (W24.write 1 S₀)._registers 24 = 1 := by rfl
+example : (W25.write 1 S₀)._registers 25 = 1 := by rfl
+example : (W26.write 1 S₀)._registers 26 = 1 := by rfl
+example : (W27.write 1 S₀)._registers 27 = 1 := by rfl
+example : (W28.write 1 S₀)._registers 28 = 1 := by rfl
+example : (W29.write 1 S₀)._registers 29 = 1 := by rfl
+example : (W30.write 1 S₀)._registers 30 = 1 := by rfl
+example : (WSP.write 1 S₀)._registers 31 = 1 := by rfl
+
+example : (W0.write 0 S₁)._registers 0 = 0 := by rfl
+example : (W1.write 0 S₁)._registers 1 = 0 := by rfl
+example : (W2.write 0 S₁)._registers 2 = 0 := by rfl
+example : (W3.write 0 S₁)._registers 3 = 0 := by rfl
+example : (W4.write 0 S₁)._registers 4 = 0 := by rfl
+example : (W5.write 0 S₁)._registers 5 = 0 := by rfl
+example : (W6.write 0 S₁)._registers 6 = 0 := by rfl
+example : (W7.write 0 S₁)._registers 7 = 0 := by rfl
+example : (W8.write 0 S₁)._registers 8 = 0 := by rfl
+example : (W9.write 0 S₁)._registers 9 = 0 := by rfl
+example : (W10.write 0 S₁)._registers 10 = 0 := by rfl
+example : (W11.write 0 S₁)._registers 11 = 0 := by rfl
+example : (W12.write 0 S₁)._registers 12 = 0 := by rfl
+example : (W13.write 0 S₁)._registers 13 = 0 := by rfl
+example : (W14.write 0 S₁)._registers 14 = 0 := by rfl
+example : (W15.write 0 S₁)._registers 15 = 0 := by rfl
+example : (W16.write 0 S₁)._registers 16 = 0 := by rfl
+example : (W17.write 0 S₁)._registers 17 = 0 := by rfl
+example : (W18.write 0 S₁)._registers 18 = 0 := by rfl
+example : (W19.write 0 S₁)._registers 19 = 0 := by rfl
+example : (W20.write 0 S₁)._registers 20 = 0 := by rfl
+example : (W21.write 0 S₁)._registers 21 = 0 := by rfl
+example : (W22.write 0 S₁)._registers 22 = 0 := by rfl
+example : (W23.write 0 S₁)._registers 23 = 0 := by rfl
+example : (W24.write 0 S₁)._registers 24 = 0 := by rfl
+example : (W25.write 0 S₁)._registers 25 = 0 := by rfl
+example : (W26.write 0 S₁)._registers 26 = 0 := by rfl
+example : (W27.write 0 S₁)._registers 27 = 0 := by rfl
+example : (W28.write 0 S₁)._registers 28 = 0 := by rfl
+example : (W29.write 0 S₁)._registers 29 = 0 := by rfl
+example : (W30.write 0 S₁)._registers 30 = 0 := by rfl
+example : (WSP.write 0 S₁)._registers 31 = 0 := by rfl
+
+example : (WREG 31).read ((WREG 31).write 1 S₀) = 0 := by rfl
+example : (WREG 31).read ((WREG 31).write 8 S₁) = 0 := by rfl
+
+-- Writing to W* overwrites the top 32-bit of X* with 0:
+example : X0.read (W0.write (1 <<< 33) allOnes) = 0 := by rfl
+example : SP.read (WSP.write 0 allOnes) = 0 := by rfl
