BignumTest/BitVec.lean
@@ -5,34 +5,35 @@ Author: Guilherme Lima
 -/
 
 import Bignum.BitVec
-
 open BitVec
 
--- toBitString
+/-! # Unit test for bitvector operations -/
+
+/-! ## toBitString -/
 
 example : (0#0).toBitString = "" := by rfl
 example : (1101#4).toBitString = "1101" := by rfl
 
--- setLsb
+/-! ## setLsb -/
 
 example : setLsb (0b0000#8) 3 true == 8#8 := by rfl
 example : setLsb (0b1010#8) 1 false == 8#8 := by rfl
 
--- extractLsb'
+/-! ## extractLsb' -/
 
-namespace extractLsb'NS
+namespace extractLsb'_NS
 def bv := 0b10010110#8
 example : bv.extractLsb' 3 2 = 2#2 := by rfl
 example : bv.extractLsb' 3 2 = bv.extractLsb'Alt 3 2 := by rfl
-end extractLsb'NS
+end extractLsb'_NS
 
--- overwriteLsb'
+/-! ## overwriteLsb' -/
 
-namespace overwriteLsb'NS
+namespace overwriteLsb'_NS
 def bv := 0b10010110#8
 example : bv.overwriteLsb' 3 2 0b01#2 = 0b10001110#8 := by rfl
 example : bv.overwriteLsb' 3 2 0b01#2 = bv.overwriteLsb'Alt 3 2 0b01#2 := by rfl
 example : bv.overwriteLsb' 0 16 0xffff = 0xffff#8 := by rfl
 example : bv.overwriteLsb' 0 16 0xffff = bv.overwriteLsb'Alt 0 16 0xffff := by rfl
 example : bv.overwriteLsb' 7 16 0x0#16 = 0b00010110#8 := by rfl
-end overwriteLsb'NS
+end overwriteLsb'_NS
